# 1.Separation of Variables
## 1.1 Cartesian Coordinate
**Example1**:
![[Untitled 3.png|Untitled 3.png]]
Two infinite grounded conducting plane remain $V=0$﻿ , closed on $yz$﻿ plane with the potential $V_0(y)$﻿. Find the potential between the two plane.

**Solution**:
The system has transformation invariance in $z$﻿ direction , thus $V$﻿ is independent of $z$﻿. And Laplace’s equation reduces to
$$\frac{\partial^2V}{\partial x^2}+\frac{\partial^2V}{\partial y^2}=0$$
subject to the boundary conditions
$$\begin{cases}V=V_0(y)&\text{when x=0}\\V\rightarrow0&\text{when x}\rightarrow\infty\end{cases}$$
**Separate the variables** **$x,y$**﻿ **into two parts** (the correctness will be discussed latter)
$$V(x,y)=X(x)\cdot Y(y)$$
Take the expression back into Laplace’s equation
$$\frac{1}{X}\frac{\partial^2X}{\partial x^2}+\frac{1}{Y}\frac{\partial^2Y}{\partial y^2}=0$$
The two parts depend on different variables completely. Therefore they must be both constant since the equation still holds when we fix one variable and change another.
$$\frac{1}{X}\frac{\partial^2X}{\partial x^2}=C_1\quad\frac{1}{Y}\frac{\partial^2Y}{\partial y^2}=-C_1$$
Generally , we need discuss the conditions $C_1$﻿ is positive or negative. But according to the boundary condition , $C_1$﻿ must be positive. Assume $C_1=k^2$﻿
$$\frac{1}{X}\frac{\partial^2X}{\partial x^2}=k^2\quad\frac{1}{Y}\frac{\partial^2Y}{\partial y^2}=-k^2$$
Solve out
$$\begin{align}X&=Ae^{kx}+Be^{-kx}\notag\\Y&=C\sin{kx}+D\cos{kx}\notag\end{align}$$
Therefore
$$V=(Ae^{kx}+Be^{-kx})\cdot(C\sin{kx}+D\cos{kx})$$
Exploit the boundary conditions
$$V=Ce^{-kx}\sin{ky}\\k=\frac{n\pi}{a}\quad(n=1,2,3\cdots)$$
As have mentioned , $\nabla^2$﻿ is a linear mapping and the solutions of Laplace’s equation is the kernal of it which is also a linear space. Therefore the general solution is a linear combination of the basis.
$$V=\sum_{n=1}^{\infty}C_ne^{-\frac{n\pi}{a}x}\sin{\frac{n\pi}{a}y}$$
Next we need determine the coefficients $C_n$﻿. According to the boundary condition
$$\sum_{n=1}^{\infty}C_n\sin{\frac{n\pi}{a}y}=V(y)$$
Actually , this is Fourier sine series , and exploit Fourier inverse transformation we can solve out
$$C_n=\frac{2}{a}\int_0^aV(y)\sin{\frac{n\pi}{a}y}$$
For example $V_0(y)=V_0$﻿ , solved
$$C_n=\begin{cases}0&\text{when n is even}\\\frac{4V_0}{n\pi}&\text{when n is odd}\end{cases}$$
Finally
$$V=\frac{4V_0}{\pi}\sum_{n=1,3\cdots}^{\infty}\frac{1}{n}e^{-\frac{n\pi}{a}x}\sin{\frac{n\pi}{a}y}$$
Now let’s pay attention to the correctness of this method. It has been proved that the functions have to have two properties to meet the separated form: **completeness** and **orthogonality**.

**Completeness**: A set of functions $f_n(y)$﻿ is said to be completed if any function $f(y)$﻿ can be expressed as a linear combination of them.
$$f(y)=\sum_{n=1}^{\infty}C_nf_n(y)$$
**Orthogonality**:A set of functions $f_n(y)$﻿ is said to be orthogonal if the integral of any two different members is zero
$$\int_0^af_n(y)f_{n'}(y)\mathrm{d}y=0 \quad(n\neq n')$$
**Example2**:
![[Untitled 1 2.png|Untitled 1 2.png]]
An infinitely long rectangular metal pipe which is closed on the $yz$﻿ plane. The potential is $V_0(y,z)$﻿ on the pipe’s ground and $0$﻿ on the wall. Find the potential in the pipe.

**Solution**:
In this case , $V$﻿ depends on all the three variables
$$\frac{\partial^2V}{\partial x^2}+\frac{\partial^2V}{\partial y^2}+\frac{\partial^2V}{\partial z^2}=0$$
And subject to the boundary conditions
$$\begin{cases}V=0&\text{when}\ y=0\ \text{or}\ a\\V=0&\text{when}\ z=0\ \text{or}\ b\\V=V_0(y,z)&\text{when}\ x=0\\V\rightarrow0&\text{when}\ x\rightarrow\infty\end{cases}$$
Similarly separate the variables $V=X(x)\cdot Y(y)\cdot Z(z)$﻿
$$\frac{1}{X}\frac{\partial^2X}{\partial x^2}+\frac{1}{Y}\frac{\partial^2Y}{\partial y^2}+\frac{1}{Z}\frac{\partial^2Z}{\partial z^2}=0$$
The three parts are both constant as the reason has been mentioned in Example1. And the parts containing $y$﻿ and $z$﻿ are negative (obviously). Assume they are $-k^2$﻿ and $-l^2$﻿ and solve
$$\begin{align}X&=A_1e^{\sqrt{k^2+l^2} x}+A_2e^{-\sqrt{k^2+l^2}x}\notag\\Y&=B_1\sin{ky}+B_2\cos{ky}\notag\\Z&=C_1\sin{lz}+C_2\cos{lz}\notag\end{align}$$
According to the boundary conditions
$$V=C_{m,n}e^{-\sqrt{(\frac{m\pi}{a})^2+(\frac{n\pi}{b})^2}x}\sin{(\frac{m\pi}{a}y)}\sin{(\frac{n\pi}{b}z)}$$
Next determine the coefficients $C_{m,n}$﻿. According to the boundary condition
$$\sum_{m=1}^{\infty}\sum_{n=1}^{\infty}C_{m,n}\sin{(\frac{m\pi}{a}y)}\sin{(\frac{n\pi}{b}z)}=V(y,z)$$
The expression is a binary Fourier transformation. Similarly we have the inverse transformation
$$C_{m,n}=\frac{4}{ab}\int_0^a\int_0^bV(y,z)\cdot\sin{(\frac{m\pi}{a}y)}\sin{(\frac{n\pi}{b}z)}\mathrm{d}y\mathrm{d}z$$
**In addition**: The **principle of superposition** and **separation of variables** can be combined to solve problems. For example, a cube with six different potentials $V_1,V_2,\cdots,V_6$﻿ on it’s faces can be seen as a superposition of six cubes with one face at potential $V_i$﻿ and others grounded.
## 1.2 Spherical Coordinate
For the system with spherical boundaries , it’s more natural to solve the problems in spherical coordinate. And Laplace’s equation reads
$$\frac{1}{r^2}\frac{\partial}{\partial r}(r^2\frac{\partial V}{\partial r})+\frac{1}{r^2\sin\theta}\frac{\partial}{\partial\theta}(\sin\theta\frac{\partial V}{\partial\theta})+\frac{1}{r^2\sin^2\theta}\frac{\partial^2V}{\partial\phi^2}=0$$
Assume the system has azimuthal symmetry: $\frac{\partial V}{\partial\phi}=0$﻿ , the equation reduces to
$$\frac{\partial}{\partial r}(r^2\frac{\partial V}{\partial r})+\frac{1}{\sin\theta}\frac{\partial}{\partial\theta}(\sin\theta\frac{\partial V}{\partial\theta})=0$$
Separate the variables in the same way:
$$\frac{1}{R}\frac{\partial}{\partial r}(r^2\frac{\partial R}{\partial r})+\frac{1}{\Theta\sin\theta}\frac{\partial}{\partial\theta}(\sin\theta\frac{\partial \Theta}{\partial\theta})=0$$
Similarly they are both constant. Assume
$$\frac{1}{R}\frac{\partial}{\partial r}(r^2\frac{\partial R}{\partial r})=l(l+1)\\\ \\\frac{1}{\Theta\sin\theta}\frac{\partial}{\partial\theta}(\sin\theta\frac{\partial \Theta}{\partial\theta})=-l(l+1)$$
For the radius equation , the general solution is
$$R=A_lr^l+\frac{B_l}{r^{l+1}}$$
However, for the angular equation, the solutions are **Legendre polynomials**
$$\Theta=P_l(\cos{\theta})$$
Legendre polynomials $P_l(x)$﻿ is defined by Rodrigues formula
$$P_l(x)=\frac{1}{2^ll!}(\frac{\mathrm{d}}{\mathrm{d}x})^l(x^2-1)^l$$
The first few Legendre polynomials are listed
$$\begin{align}P_0(x)&=1\notag\\P_1(x)&=x\notag\\P_2(x)&=\frac{1}{2}(3x^2-1)\notag\\P_3(x)&=\frac{1}{2}(5x^3-3x)\notag\\P_4(x)&=\frac{1}{8}(35x^4-30x^2+3)\notag\end{align}$$
Some properties: $P_l(x)$﻿ is a $l$﻿th-order polynomial in $x$﻿, and only contains even(odd) power if $l$﻿ is even(odd). The factor in front $\frac{1}{2^ll!}$﻿ was chosen in order that $P_l(1)=1$﻿

And one more confusion: A second-order differential equation has two independent solutions, what about another solution? Actually “another solution” will blow up at $\theta=0$﻿ or $\theta=\pi$﻿

Therefore, a general separable solution
$$V_l=(A_lr^l+\frac{B_l}{r^{l+1}})P_l(\cos\theta)$$
And the general solution is a linear combination of them
$$V=\sum_{l=1}^{\infty}(A_lr^l+\frac{B_l}{r^{l+1}})P_l(\cos\theta)$$
Similar to Fourier sine series, Legendre polynomials have completeness and orthogonality
$$\begin{align}\int_{-1}^1P_l(x)P_{l'}(x)\mathrm{d}x&=\int_0^{\pi}P_l(\cos\theta)P_{l'}(\cos\theta)\sin\theta\mathrm{d}\theta\notag\\&=\begin{cases}0&\text{if}\ l\neq l'\\\frac{2}{2l+1}&\text{if}\ l=l'\end{cases}\notag\end{align}$$
This is used to determine $A_l$﻿ and $B_l$﻿.
**In addition**: if $V$﻿ depends on all the three variables, the general solution becomes
$$V=\sum_{l=1}^{\infty}(A_lr^l+\frac{B_l}{r^{l+1}})\cdot P_l(\cos\theta)\cdot(C_l\sin{l\phi}+D_l\cos{l\phi})$$
**Example1**: $V_0(\theta)$﻿ is specific on a spherical shell with radius $R$﻿, find the potential inside and outside the surface.
**Solution**:
**Inside**: $B_l$﻿ must be zero or it will blow up at origin
$$V=\sum_{l=1}^{\infty}A_lr^lP_l(\cos\theta)$$
According to the boundary condition on the surface
$$\sum_{l=1}^{\infty}A_lR^lP_l(\cos\theta)=V_0(\theta)$$
Exploit the orthogonality to determine $A_l$﻿
$$A_l=\frac{2l+1}{2R^l}\int_0^{\pi}V_0(\theta)P_l(\cos\theta)\sin\theta\mathrm{d}\theta$$
**Outside**: $A_l=0$﻿
$$V=\sum_{l=0}^{\infty}\frac{B_l}{r^{l+1}}P_l(\cos\theta)$$
And
$$B_l=\frac{2l+1}{2}R^{l+1}\int_0^{\pi}V_0(\theta)P_l(\cos\theta)\sin\theta\mathrm{d}\theta$$
Usually we won’t integrate directly

**Example2**:
![[Untitled 2 2.png|Untitled 2 2.png]]
A classical model: A grounded conducting spherical shell is placed in an uniform electric field. Find the potential outside the shell and the charge density $\sigma(\theta)$﻿ on the surface.
**Solution**:
The boundary conditions of this system:
$$\begin{cases}V=0&\text{when}\ r=R\\V\rightarrow-E_0rcos\theta&\text{when}\ r\gg R\end{cases}$$
Therefore the general solution consists two parts
$$V=V_1+V_2\\\begin{cases}V_1=-E_0r\cos\theta\\V_2=\sum_{l=0}^{\infty}\frac{B_l}{r^{l+1}}P_l(\cos\theta)\end{cases}$$
Exploit the boundary condition
$$\sum_{l=0}^{\infty}\frac{B_l}{R^{l+1}}P_l(\cos\theta)=E_0R\cos\theta$$
Solve out
$$B_l=\begin{cases}E_0R^3&\text{when}\ l=1\\0&\text{when}\ l\neq0\end{cases}$$
Therefore the complete potential is
$$V=(\frac{R^3}{r^2}-r)E_0\cos\theta$$
Next determine the charge density on the surface
$$\begin{align}\sigma(\theta)&=-\epsilon_0\left.\frac{\partial V}{\partial r}\right|_{r=R}\notag\\&=3\epsilon_0E_0\cos\theta\notag\end{align}$$

**Example3**: The surface charge density $\sigma(\theta)$﻿ is specific on a spherical shell. Find the potential inside and outside the surface.
**Solution**:
Actually, $\sigma(\theta)$﻿ indicates the partial derivate $\frac{\partial V}{\partial r}$﻿ on the surface.
$$\begin{align*}\text{inside: }V_{\text{in}}&=\sum_{l=1}^{\infty}A_lr^lP_l(\cos\theta)\\\text{outside: }V_{\text{out}}&=\sum_{l=1}^{\infty}\frac{B_l}{r^{l+1}}P_l(\cos\theta)\end{align*}$$
For the charge density on a surface, we have the formula
$$\sigma=-\epsilon_0(\frac{\partial V_{\text{out}}}{\partial r}-\frac{\partial V_{\text{in}}}{\partial r})$$
Take the expression of $V_{\text{out}}$﻿ and $V_{\text{in}}$﻿ into the formula
$$\sum_{l=1}^{\infty}\left(lA_lR^{l-1}+(l+1)\frac{B_l}{R^{l+2}}\right)P_l(\cos\theta)={\sigma(\theta)\over\epsilon_0}$$
Simultaneously, the potential is continuous on the boundary
$$A_lR^l=\frac{B_l}{R^{l+1}}$$
Therefore we can solve out
$$A_l=\frac{1}{2\epsilon_0R^{l-1}}\int_0^\pi\sigma(\theta)P_l(\cos\theta)\sin\theta\mathrm{d}\theta\\\ \\B_l=\frac{1}{2\epsilon_0}R^{l+2}\int_0^\pi\sigma(\theta)P_l(\cos\theta)\sin\theta\mathrm{d}\theta$$
## 1.3 Cylindrical Coordinate
In cylindrical coordinate, the form of Laplace’s equation becomes
$$\frac{1}{s}\frac{\partial}{\partial s}(s\frac{\partial V}{\partial s})+\frac{1}{s^2}\frac{\partial^2V}{\partial \phi^2}+\frac{\partial^2V}{\partial z^2}=0$$
Generally, the system we consider has the cylindrical symmetry, so that $V$﻿ is independent of $z$﻿. Similarly separate the variables $s$﻿ and $\phi$﻿: $V=S(s)\cdot\Phi(\phi)$﻿
$$\frac{s}{S}\frac{\partial}{\partial s}(s\frac{\partial S}{\partial s})+\frac{1}{\Phi}\frac{\partial^2\Phi}{\partial \phi^2}=0$$
They are both constant. Assume the first part is equal to $k^2$﻿ and the second negative
$$\begin{align*}\frac{\partial}{\partial s}(s\frac{\partial S}{\partial s})=\frac{k^2}{s}S\\\ \\\frac{\partial^2\Phi}{\partial \phi^2}=-k^2\Phi\end{align*}$$
The general solutions:
$$\begin{align*}S&=\begin{cases}A\ln{s}+B&\text{when }k=0\\C_ks^k+D_ks^{-k}&\text{when }k\neq0\end{cases}\\\ \\\Phi&=E_k\sin{k\phi}+F_k\cos{k\phi}\end{align*}$$
Therefore, the completed solution is a linear combination of them
$$V=A\ln{s}+B+\sum_{k=1}^{\infty}(C_ks^k+D_ks^{-k})\cdot(E_k\sin{k\phi}+F_k\cos{k\phi})$$

**Example**:
![[Untitled 2 2.png|Untitled 2 2.png]]
A infinitely long grounded metal pipe of radius $R$﻿ is placed in a uniform electric field $E_0$﻿. Find the potential outside the pipe and the charge density on the surface.
**Solution**:
In this system, the potential consists two parts: the origin potential and that produced by the induced charges.
$$V=V_1+V_2\\V_1=-E_0s\cos\phi\\V_2=A\ln{s}+B+\sum_{k=1}^{\infin}(C_ks^k+D_ks^{-k})\cdot(E_k\sin{k\phi}+F_k\cos{k\phi})$$
The boundary conditions
$$\begin{cases}V=0&\text{when }s=R\\V\rightarrow0&\text{when }s\rightarrow\infty\end{cases}$$
Exploit the boundary conditions, $A$﻿, $B$﻿ and $C_k$﻿ are all zero.
$$V_2=\frac{E_0R^2}{s}\cos\phi$$
Therefore the complete potential is
$$V=(\frac{R^2}{s}-s)E_0\cos{\phi}$$
Then we can get the charge density on the surface
$$\begin{align*}\sigma(\theta)&=-\epsilon_0(\left.\frac{\partial V_{\text{out}}}{\partial s}\right|_{s=R}-\left.\frac{\partial V_{\text{in}}}{\partial s}\right|_{s=R})\\&=2\epsilon_0E_0\cos\phi\end{align*}$$
# 2.Multipole Expansion
## 2.1 Approximate Potential at Large Distance
Consider the space very far from the localized charges distributions, the most approximate expression of the potential is $\frac{Q}{4\pi\epsilon_0r}$﻿. But when $Q=0$﻿, we have to take into account the higher-order terms.

**Example**:(A physical dipole) Two charges with the same magnitude $q$﻿ and opposite sign are placed at a distance $d$﻿. Find the potential in the space far from the dipole.
Solution:
$$V=\frac{q}{4\pi\epsilon_0}(\frac{1}{r_{+}}-\frac{1}{r_-})$$
and
$$\begin{align*}r_+=(r^2+\frac{1}{4}d^2-dr\cos{\theta})^{\frac{1}{2}}\\r_-=(r^2+\frac{1}{4}d^2+dr\cos{\theta})^{\frac{1}{2}}\end{align*}$$
Expand them to the first-order
$$\frac{1}{r_{+}}-\frac{1}{r_-}=\frac{d\cos\theta}{r^2}$$
Therefore, the potential is
$$V=\frac{qd\cos\theta}{4\pi\epsilon_0r^2}$$
And is corresponding to the power of $\frac{1}{r}$﻿

| Monopole   | $V\thicksim\frac{1}{r}$   |
| ---------- | ------------------------- |
| Dipole     | $V\thicksim\frac{1}{r^2}$ |
| Quadrupole | $V\thicksim\frac{1}{r^3}$ |
| Octopole   | $V\thicksim\frac{1}{r^4}$ |

**A systematic expansion for any localized charge distribution**:
The general expression of the potential
$$V=\frac{1}{4\pi\epsilon_0}\int\frac{1}{|\vec{r}-\vec{r}'|}\rho(\vec{r}')\mathrm{d}\tau'$$
Because $r\gg r'$﻿, $\frac{1}{|\vec{r}-\vec{r}'|}$﻿ can be expanded to be
$$\frac{1}{|\vec{r}-\vec{r}'|}=\frac{1}{r}\left(1+\cos\alpha\frac{r'}{r}+\frac{1}{2}(3\cos^2\alpha-1)(\frac{r'}{r})^2+\frac{1}{2}(5\cos^3\alpha -3\cos\alpha)(\frac{r'}{r})^3+\cdots\right)$$
The expression is equivalent to
$$\frac{1}{|\vec{r}-\vec{r}'|}=\frac{1}{r}\sum_{l=0}^{\infty}(\frac{r'}{r})^{l}P_l(\cos\alpha)$$
Therefore the expression of $V$﻿ is
$$V=\frac{1}{4\pi\epsilon_0}\sum_{l=0}^{\infty}\frac{1}{r^{l+1}}\int(r')^{l}\rho(\vec{r}')P_l(\cos\alpha)\mathrm{d}\tau'$$
The key to computer each term is to distinguish the angle $\alpha$﻿ and those in the localized distribution.
## 2.2 The Dipole and Quadrupole
Take a look into the first few terms of the expression of $V$﻿
$$V=\frac{1}{4\pi\epsilon_0}\left(\frac{1}{r}\int\rho(r')\mathrm{d}\tau'+\frac{1}{r^2}\int r'\rho(r')P_1(\cos\alpha)\mathrm{d}\tau'+\frac{1}{r^3}\int(r')^2\rho(r')P_2(\cos\alpha)\mathrm{d}\tau'+\cdots\right)$$
Obviously, $\int\rho(r')\mathrm{d}\tau'=Q$﻿ and $V_{\text{mono}}=\frac{Q}{4\pi\epsilon_0 r}$﻿(the same as a point charge).
If the total charge $Q$﻿ is zero, the dipole will take the dominant term.
$$\begin{align*}V&=\frac{1}{4\pi\epsilon_0}\cdot\frac{1}{r^2}\int r'\rho(r')P_1(\cos\alpha)\mathrm{d}\tau'\\&=\frac{1}{4\pi\epsilon_0r^3}(\vec{r}\cdot\int\vec{r}'\rho(r')\mathrm{d}\tau')\end{align*}$$
The integral is called **the dipole moment** $\vec{p}$﻿
$$\vec{p}=\int\vec{r}'\rho(r')\mathrm{d}\tau'$$
ant the potential can be expressed as
$$V_{\text{dip}}=\frac{\vec{p}\cdot\vec{r}}{4\pi\epsilon_0r^3}$$
Moreover, if $\vec{p}=0$﻿, we have to consider the quadrupole term
$$V_{\text{quad}}=\frac{1}{4\pi\epsilon_0r^3}\int(r')^3\rho(r')P_2(\cos\alpha)\mathrm{d}\tau'$$
If we expand $V$﻿ in another way, we will get
$$V_{\text{quad}}=\frac{1}{4\pi\epsilon_0}\cdot\frac{1}{2r^5}\overleftrightarrow{D}:\vec{r}\vec{r}$$
where
$$\overleftrightarrow{D}=\int\rho(r')(3\vec{r'}\vec{r'}-r'^2\overleftrightarrow{I})\mathrm{d}\tau'$$
is called **the quadrupole moment**
## 2.3 Origin of Coordinate in Multipole Expansion
The dipole moment is dependent of the origin.  
Suppose the system has a total charge  
$Q$﻿ and dipole moment $\vec{p}$﻿ in the original coordinate. Then displace the origin by $\vec{a}$﻿ and get the new cooridinate.  
The new dipole moment  
$$\begin{align*}\vec{p}'&=\int\vec{r}'\rho(r')\mathrm{d}\tau'=\int(\vec{r}-\vec{a})\rho(r)\mathrm{d}\tau\\&=\vec{p}-Q\vec{a}\end{align*}$$
In particular, if $Q=0$﻿, $\vec{p}$﻿ is independent of the origin.